phoas?

synth.v
@@ -6,6 +6,9 @@ Import ListNotations MonadNotation.
 Require Export Coq.Strings.String.
 Require Import Ascii.
 Extraction Language Haskell.
+Require Import FMaps.
+Require Import ExtLib.Data.HList.
+
 
 Definition printInductive (name  : ident): TemplateMonad unit :=
   (tmBind (tmQuoteInductive name) tmPrint).
@@ -22,7 +25,153 @@ Inductive b : Type :=
 | Ba : a -> b
 | Baa : a -> b -> b.
 
-Run TemplateProgram (t <- tmQuoteInductive "b";; tmPrint t).
+Inductive prod3 (A B C : Type) : Type := 
+pair3 : A -> B -> prod3 A B C
+| pair3' : B -> prod3 A B C
+| pair3'' : C -> prod3 A B C.
+
+Print sum.
+Definition rec (F : Type -> Type -> Type) (A : Type) : Type := forall X, (F X A -> X) -> X.
+
+Definition snat := rec (fun X _ => sum unit X) unit.
+
+Definition szero : snat := fun x f => f (inl tt).
+Definition sone : snat := fun x f => f (inr (szero x f)).
+
+Definition twice (sn : snat) : snat := fun x f => 
+sn x (fun body => 
+match body with
+| inl tt => f (inl tt)
+| inr n' => f (inr (f (inr (n'))))
+end).
+
+Definition ss (sn : snat) : snat := fun x f => f (inr (sn x f)).
+
+Definition list' := rec (fun X A => sum unit (prod A X)).
+
+
+Goal ss szero = sone.
+Proof.
+compute. reflexivity.
+Qed.
+
+Check (fun t1 t2 => prod (list t1) (list (list t2))).
+Inductive TyOp : Type := 
+| tfunctor : forall (F : Type -> Type), TyOp
+| tprod : TyOp -> TyOp -> TyOp
+| tsum : TyOp -> TyOp -> TyOp.
+
+
+
+Section var.
+Variable var : (Type -> Type) -> Type.
+
+
+Inductive Species : (Type -> Type) -> Type := 
+| zero : Species (fun _ => Empty_set)
+| one : Species (fun x => unit)
+| singleton : Species (fun x => x)
+| cprod : forall {F G}, Species F -> Species G -> Species (fun x => prod (F x) (G x))
+| ssum : forall {F G}, Species F -> Species G -> Species (fun x => sum (F x) (G x))
+| srec : forall F, (forall A, (var (F A) -> Species (F A))) -> Species (rec F)
+| svar : forall F, var F -> Species F.
+End var.
+
+Check Species.
+
+Definition var1 := fun _ : Type -> Type => unit.
+Definition F1 := (fun A X => sum unit (prod A X)).
+Definition Id := fun X : Type => X.
+
+
+Definition s1 := (srec var1 F1 (fun A v => ssum var1 (one var1) (cprod var1 (singleton var1) (svar var1 Id v)))).
+
+Definition split_i {X : Type} (i : nat) (l : list X) := (firstn i l, skipn i l).
+
+Fixpoint tabulate_list {X : Type} (f : nat -> X) n := 
+match n with 
+| 0 => []
+| S n => cons (f n) (tabulate_list f n)
+end.
+
+Check 4::[].
+
+Definition varType n' n bound (T1 T2 : Type) : Type := 
+match existsb (fun e => e =? n') bound with 
+  | false => T1
+  | _ => 
+    match n' =? n with 
+    | true => T2
+    | _ => T1
+    end
+  end.
+
+Definition varExp {T1 T2} n' n bound (E1 : T1) (E2 : T2) : varType n' n bound T1 T2 :=
+match existsb (fun e => e =? n') bound as r return 
+match r with 
+|false => T1
+| _ => match n' =? n with 
+        | true => T2
+        | _ => T1 end
+end
+with 
+  | false => E1
+  | _ => 
+    match n' =? n as r' return 
+    match r' with 
+    | true => T2
+    | _ => T1
+    end
+   with 
+    | true => E2
+    | _ => E1
+    end
+  end.
+
+Fixpoint squash var T (s : Species (Species var) T) : Species var T :=
+match s with 
+| zero _ => zero _
+| one _ => one _
+| singleton _ _ => singleton _ _
+| cprod _ T1 T2 => cprod _ (squash var _ T1) (squash var _ T2)
+| ssum _ T1 T2 => ssum _ (squash var _ T1) (squash var _ T2)
+| srec _ F f => srec _ F (fun A v => squash var _ (f A (svar var (F A) v)))
+| svar _ F v => v
+end.
+
+Definition Species1 (t1 t2 : Type -> Type) := forall v, v t1 -> Species v t2.
+
+Definition Subst {var} (t1 t2 : Type -> Type) (T : Species1 t1 t2) (T' : Species var t1) : Species var t2 :=  
+squash var _ (T (Species var) T').
+
+Fixpoint enumerate A S s labels := 
+let fix enum (A : Type) {var} {S : Type -> Type} (s : Species var S) (labels : list A) : list (S A) := 
+match s with
+| zero _ => []
+| (one _) => match labels with [] => [tt ] | _ => [] end
+| singleton _ => match labels with [x] => [x] | _ => [] end
+| cprod _  s1 s2 => 
+  let all_splits := map (fun i => split_i i labels) (tabulate_list (fun i => i) (List.length labels)) in 
+  concat (map (fun e => match e with (l,r) => list_prod (enum A s1 l) (enum A s2 r) end) all_splits)
+| ssum _ s1 s2 => app (map inl (enum A s1 labels)) (map inr (enum A s2 labels))
+| srec _ F f => 
+  let body := Subst _ _ (f A) s 
+  in enum A (F A) body labels
+| svar _ F v => []
+end
+in 
+enum A S s labels.
+
+Compute enumerate nat (rec (fun t => t) (fun x =>
+match x with
+| interp F => ssum one (cprod singleton (var F))
+end)) [1;2]. 
+
+Compute enumerate nat (cprod (ssum singleton singleton) (ssum singleton singleton)) [1;2].
+
+Print list.
+
+Run TemplateProgram (t <- tmQuoteRec (list nat);; r <- tmEval all t;; tmPrint r).
 
 Run TemplateProgram (t<- (tmQuote (nat -> nat));; t <- tmUnquoteTyped Set t;; tmPrint t).
 
@@ -59,6 +208,8 @@ end.
 Compute strip "Coq.Init.Datatypes.nat" 100.
  
 Check fold_left.
+
+Print prod.
 
 Fixpoint enumerate (ind : Type) (n : nat) : TemplateMonad (list ind) := 
 tm <- tmQuote ind;; match tm with 
@@ -128,19 +279,12 @@ match n with
 | S n => S.add (f n) (tabulate f n)
 end.
 
-Fixpoint tabulate_list {X : Type} (f : nat -> X) n := 
-match n with 
-| 0 => []
-| S n => cons (f n) (tabulate_list f n)
-end.
-
 Definition list_max {X : Type} (f : X -> X -> bool) l d := fold_left (fun acc e => if f acc e then acc else e) l d.
 
 Fixpoint all_subset (s : S.t) := 
 S.fold (fun e subsets => subsets ++ (map (fun s => S.add e s) subsets)) s [S.empty].
 
 
-Definition split_i {X : Type} (i : nat) (l : list X) := (firstn i l, skipn i l).
 
 Fixpoint all_perm {X : Type} (l : list X) :=
 match l with 
